feat: use vectors

Batteries/Data/BinaryHeap.lean
@@ -1,78 +1,85 @@
 /-
 Copyright (c) 2021 Mario Carneiro. All rights reserved.
 Released under Apache 2.0 license as described in the file LICENSE.
-Authors: Mario Carneiro
+Authors: Mario Carneiro, François G. Dorais
 -/
+
+import Batteries.Data.Vector.Basic
 
 namespace Batteries
 
 /-- A max-heap data structure. -/
 structure BinaryHeap (α) (lt : α → α → Bool) where
-  /-- Backing array for `BinaryHeap`. -/
+  /-- `O(1)`. Get data array for a `BinaryHeap`. -/
   arr : Array α
 
 namespace BinaryHeap
 
-/-- Core operation for binary heaps, expressed directly on arrays.
-Given an array which is a max-heap, push item `i` down to restore the max-heap property. -/
-def heapifyDown (lt : α → α → Bool) (a : Array α) (i : Fin a.size) :
-    {a' : Array α // a'.size = a.size} :=
+private def maxChild (lt : α → α → Bool) (a : Vector α sz) (i : Fin sz) : Option (Fin sz) :=
   let left := 2 * i.1 + 1
   let right := left + 1
-  have left_le : i ≤ left := Nat.le_trans
-    (by rw [Nat.succ_mul, Nat.one_mul]; exact Nat.le_add_left i i)
-    (Nat.le_add_right ..)
-  have right_le : i ≤ right := Nat.le_trans left_le (Nat.le_add_right ..)
-  have i_le : i ≤ i := Nat.le_refl _
-  have j : {j : Fin a.size // i ≤ j} := if h : left < a.size then
-    if lt (a.get i) (a.get ⟨left, h⟩) then ⟨⟨left, h⟩, left_le⟩ else ⟨i, i_le⟩ else ⟨i, i_le⟩
-  have j := if h : right < a.size then
-    if lt (a.get j) (a.get ⟨right, h⟩) then ⟨⟨right, h⟩, right_le⟩ else j else j
-  if h : i.1 = j then ⟨a, rfl⟩ else
-    let a' := a.swap i j
-    let j' := ⟨j, by rw [a.size_swap i j]; exact j.1.2⟩
-    have : a'.size - j < a.size - i := by
-      rw [a.size_swap i j]; exact Nat.sub_lt_sub_left i.2 <| Nat.lt_of_le_of_ne j.2 h
-    let ⟨a₂, h₂⟩ := heapifyDown lt a' j'
-    ⟨a₂, h₂.trans (a.size_swap i j)⟩
-termination_by a.size - i
+  if hleft : left < sz then
+    if hright : right < sz then
+      if lt a[left] a[right] then
+        some ⟨right, hright⟩
+      else
+        some ⟨left, hleft⟩
+    else
+      some ⟨left, hleft⟩
+  else none
 
-@[simp] theorem size_heapifyDown (lt : α → α → Bool) (a : Array α) (i : Fin a.size) :
-    (heapifyDown lt a i).1.size = a.size := (heapifyDown lt a i).2
+/-- Core operation for binary heaps, expressed directly on arrays.
+Given an array which is a max-heap, push item `i` down to restore the max-heap property. -/
+def heapifyDown (lt : α → α → Bool) (a : Vector α sz) (i : Fin sz) :
+    Vector α sz :=
+  match h : maxChild lt a i with
+  | none => a
+  | some j =>
+    have : i < j := by
+      cases i; cases j
+      simp only [maxChild] at h
+      split at h
+      · split at h
+        · split at h <;> (cases h; simp_arith)
+        · cases h; simp_arith
+      · contradiction
+    if lt a[i] a[j] then
+      heapifyDown lt (a.swap i j) j
+    else a
+termination_by sz - i
 
 /-- Core operation for binary heaps, expressed directly on arrays.
 Construct a heap from an unsorted array, by heapifying all the elements. -/
-def mkHeap (lt : α → α → Bool) (a : Array α) : {a' : Array α // a'.size = a.size} :=
+def mkHeap (lt : α → α → Bool) (a : Vector α sz) : Vector α sz :=
   loop (a.size / 2) a (Nat.div_le_self ..)
 where
   /-- Inner loop for `mkHeap`. -/
-  loop : (i : Nat) → (a : Array α) → i ≤ a.size → {a' : Array α // a'.size = a.size}
-  | 0, a, _ => ⟨a, rfl⟩
+  loop : (i : Nat) → (a : Vector α sz) → i ≤ sz → Vector α sz
+  | 0, a, _ => a
   | i+1, a, h =>
-    let h := Nat.lt_of_succ_le h
-    let a' := heapifyDown lt a ⟨i, h⟩
-    let ⟨a₂, h₂⟩ := loop i a' ((heapifyDown ..).2.symm ▸ Nat.le_of_lt h)
-    ⟨a₂, h₂.trans a'.2⟩
+    let a' := heapifyDown lt a ⟨i, Nat.lt_of_succ_le h⟩
+    loop i a' (Nat.le_trans (Nat.le_succ _) h)
 
-@[simp] theorem size_mkHeap (lt : α → α → Bool) (a : Array α) :
-    (mkHeap lt a).1.size = a.size := (mkHeap lt a).2
+private def parent : Fin sz → Option (Fin sz)
+  | ⟨0, _⟩ => none
+  | ⟨i+1, hi⟩ => some ⟨i / 2, Nat.lt_of_le_of_lt (Nat.div_le_self _ _) (Nat.lt_of_succ_lt hi)⟩
 
 /-- Core operation for binary heaps, expressed directly on arrays.
 Given an array which is a max-heap, push item `i` up to restore the max-heap property. -/
-def heapifyUp (lt : α → α → Bool) (a : Array α) (i : Fin a.size) :
-    {a' : Array α // a'.size = a.size} :=
-  if i0 : i.1 = 0 then ⟨a, rfl⟩ else
-    have : (i.1 - 1) / 2 < i := Nat.lt_of_le_of_lt (Nat.div_le_self ..) <|
-      Nat.sub_lt (Nat.pos_of_ne_zero i0) Nat.zero_lt_one
-    let j := ⟨(i.1 - 1) / 2, Nat.lt_trans this i.2⟩
-    if lt (a.get j) (a.get i) then
-      let a' := a.swap i j
-      let ⟨a₂, h₂⟩ := heapifyUp lt a' ⟨j.1, by rw [a.size_swap i j]; exact j.2⟩
-      ⟨a₂, h₂.trans (a.size_swap i j)⟩
-    else ⟨a, rfl⟩
-
-@[simp] theorem size_heapifyUp (lt : α → α → Bool) (a : Array α) (i : Fin a.size) :
-    (heapifyUp lt a i).1.size = a.size := (heapifyUp lt a i).2
+def heapifyUp (lt : α → α → Bool) (a : Vector α sz) (i : Fin sz) :
+    Vector α sz :=
+  match h : parent i with
+  | none => a
+  | some j =>
+    have : j < i := by
+      cases i; cases j
+      simp only [parent] at h
+      split at h
+      · contradiction
+      · next heq => cases heq; cases h; simp_arith [Nat.div_le_self]
+    if lt a[j] a[i] then
+      heapifyUp lt (a.swap i j) j
+    else a
 
 /-- `O(1)`. Build a new empty heap. -/
 def empty (lt) : BinaryHeap α lt := ⟨#[]⟩
@@ -86,81 +93,91 @@ def singleton (lt) (x : α) : BinaryHeap α lt := ⟨#[x]⟩
 /-- `O(1)`. Get the number of elements in a `BinaryHeap`. -/
 def size (self : BinaryHeap α lt) : Nat := self.1.size
 
+/-- `O(1)`. Get data vector of a `BinaryHeap`. -/
+def vector (self : BinaryHeap α lt) : Vector α self.size := ⟨self.1, rfl⟩
+
 /-- `O(1)`. Get an element in the heap by index. -/
 def get (self : BinaryHeap α lt) (i : Fin self.size) : α := self.1.get i
 
 /-- `O(log n)`. Insert an element into a `BinaryHeap`, preserving the max-heap property. -/
 def insert (self : BinaryHeap α lt) (x : α) : BinaryHeap α lt where
-  arr := let n := self.size;
-    heapifyUp lt (self.1.push x) ⟨n, by rw [Array.size_push]; apply Nat.lt_succ_self⟩
+  arr := heapifyUp lt (self.vector.push x) ⟨_, Nat.lt_succ_self _⟩ |>.toArray
 
 @[simp] theorem size_insert (self : BinaryHeap α lt) (x : α) :
     (self.insert x).size = self.size + 1 := by
-  simp [insert, size, size_heapifyUp]
+  simp only [insert, size, Vector.size_eq]
 
 /-- `O(1)`. Get the maximum element in a `BinaryHeap`. -/
-def max (self : BinaryHeap α lt) : Option α := self.1.get? 0
-
-/-- Auxiliary for `popMax`. -/
-def popMaxAux (self : BinaryHeap α lt) : {a' : BinaryHeap α lt // a'.size = self.size - 1} :=
-  match e: self.1.size with
-  | 0 => ⟨self, by simp [size, e]⟩
-  | n+1 =>
-    have h0 := by rw [e]; apply Nat.succ_pos
-    have hn := by rw [e]; apply Nat.lt_succ_self
-    if hn0 : 0 < n then
-      let a := self.1.swap ⟨0, h0⟩ ⟨n, hn⟩ |>.pop
-      ⟨⟨heapifyDown lt a ⟨0, by rwa [Array.size_pop, Array.size_swap, e]⟩⟩,
-        by simp [size, a]⟩
-    else
-      ⟨⟨self.1.pop⟩, by simp [size]⟩
+def max (self : BinaryHeap α lt) : Option α := self.1[0]?
 
 /-- `O(log n)`. Remove the maximum element from a `BinaryHeap`.
 Call `max` first to actually retrieve the maximum element. -/
-def popMax (self : BinaryHeap α lt) : BinaryHeap α lt := self.popMaxAux
+def popMax (self : BinaryHeap α lt) : BinaryHeap α lt :=
+  if h0 : self.size = 0 then self else
+    have hs : self.size - 1 < self.size := Nat.pred_lt h0
+    have h0 : 0 < self.size := Nat.zero_lt_of_ne_zero h0
+    let v := self.vector.swap ⟨_, h0⟩ ⟨_, hs⟩ |>.pop
+    if h : 0 < v.size then
+      ⟨heapifyDown lt v ⟨0, h⟩ |>.toArray⟩
+    else
+      ⟨v.toArray⟩
 
 @[simp] theorem size_popMax (self : BinaryHeap α lt) :
-    self.popMax.size = self.size - 1 := self.popMaxAux.2
+    self.popMax.size = self.size - 1 := by
+  simp only [popMax, size]
+  split
+  · simp_arith [*]
+  · split <;> simp_arith [Vector.size_eq, *]
 
 /-- `O(log n)`. Return and remove the maximum element from a `BinaryHeap`. -/
 def extractMax (self : BinaryHeap α lt) : Option α × BinaryHeap α lt :=
   (self.max, self.popMax)
 
-theorem size_pos_of_max {self : BinaryHeap α lt} (e : self.max = some x) : 0 < self.size :=
-  Decidable.of_not_not fun h : ¬ 0 < self.1.size => by simp [BinaryHeap.max, Array.get?, h] at e
+theorem size_pos_of_max {self : BinaryHeap α lt} (h : self.max = some x) : 0 < self.size := by
+  simp only [max, GetElem.getElem?] at h
+  split at h
+  · assumption
+  · contradiction
 
 /-- `O(log n)`. Equivalent to `extractMax (self.insert x)`, except that extraction cannot fail. -/
 def insertExtractMax (self : BinaryHeap α lt) (x : α) : α × BinaryHeap α lt :=
-  match e: self.max with
+  match e : self.max with
   | none => (x, self)
   | some m =>
     if lt x m then
-      let a := self.1.set ⟨0, size_pos_of_max e⟩ x
-      (m, ⟨heapifyDown lt a ⟨0, by simp only [Array.size_set, a]; exact size_pos_of_max e⟩⟩)
+      let v := self.vector.set ⟨0, size_pos_of_max e⟩ x
+      (m, ⟨heapifyDown lt v ⟨0, size_pos_of_max e⟩ |>.toArray⟩)
     else (x, self)
 
 /-- `O(log n)`. Equivalent to `(self.max, self.popMax.insert x)`. -/
 def replaceMax (self : BinaryHeap α lt) (x : α) : Option α × BinaryHeap α lt :=
-  match e: self.max with
-  | none => (none, ⟨self.1.push x⟩)
+  match e : self.max with
+  | none => (none, ⟨self.vector.push x |>.toArray⟩)
   | some m =>
-    let a := self.1.set ⟨0, size_pos_of_max e⟩ x
-    (some m, ⟨heapifyDown lt a ⟨0, by simp only [Array.size_set, a]; exact size_pos_of_max e⟩⟩)
+    let v := self.vector.set ⟨0, size_pos_of_max e⟩ x
+    (some m, ⟨heapifyDown lt v ⟨0, size_pos_of_max e⟩ |>.toArray⟩)
 
 /-- `O(log n)`. Replace the value at index `i` by `x`. Assumes that `x ≤ self.get i`. -/
 def decreaseKey (self : BinaryHeap α lt) (i : Fin self.size) (x : α) : BinaryHeap α lt where
-  arr := heapifyDown lt (self.1.set i x) ⟨i, by rw [self.1.size_set]; exact i.2⟩
+  arr := heapifyDown lt (self.vector.set i x) i |>.toArray
 
 /-- `O(log n)`. Replace the value at index `i` by `x`. Assumes that `self.get i ≤ x`. -/
 def increaseKey (self : BinaryHeap α lt) (i : Fin self.size) (x : α) : BinaryHeap α lt where
-  arr := heapifyUp lt (self.1.set i x) ⟨i, by rw [self.1.size_set]; exact i.2⟩
+  arr := heapifyUp lt (self.vector.set i x) i |>.toArray
 
 end Batteries.BinaryHeap
 
+/-- `O(n)`. Convert an unsorted vector to a `BinaryHeap`. -/
+def Batteries.Vector.toBinaryHeap (lt : α → α → Bool) (v : Vector α n) :
+    Batteries.BinaryHeap α lt where
+  arr := BinaryHeap.mkHeap lt v |>.toArray
+
+open Batteries in
 /-- `O(n)`. Convert an unsorted array to a `BinaryHeap`. -/
 def Array.toBinaryHeap (lt : α → α → Bool) (a : Array α) : Batteries.BinaryHeap α lt where
-  arr := Batteries.BinaryHeap.mkHeap lt a
+  arr := BinaryHeap.mkHeap lt ⟨a, rfl⟩ |>.toArray
 
+open Batteries in
 /-- `O(n log n)`. Sort an array using a `BinaryHeap`. -/
 @[specialize] def Array.heapSort (a : Array α) (lt : α → α → Bool) : Array α :=
   loop (a.toBinaryHeap (flip lt)) #[]
